WIP Code generation

Uppaal_Networks/UPPAAL_Asm_AbsInt.thy
@@ -175,8 +175,19 @@ instance proof
 qed
 end
 
-class absstate = complete_lattice
-instantiation state_map :: (absstate) absstate begin instance proof qed end
+class is_bot = bot +
+  fixes is_bot :: "'a \<Rightarrow> bool"
+  assumes is_bot: "is_bot a \<longleftrightarrow> (a = \<bottom>)"
+
+class absstate = complete_lattice + is_bot
+
+instantiation state_map :: (absstate) absstate (*begin instance .. end*)
+begin
+definition "is_bot_state_map (a::'a state_map) = (a = \<bottom>)"
+instance proof
+  show "is_bot a \<longleftrightarrow> (a::'a state_map) = \<bottom>" for a by (simp add: is_bot_state_map_def)
+qed
+end
 
 subsection "Abstract Stepping"
 
@@ -441,6 +452,7 @@ proof -
 qed
 
 definition[simp]: "ai_loop \<equiv> loop ai_step"
+
 theorem ai_loop_correct: "collect_loop prog n (\<gamma>_map entry) \<le> \<gamma>_map (ai_loop prog n entry)"
 proof (induction n arbitrary: entry)
   case 0
