Uppaal_Networks/UPPAAL_Asm_AbsInt_State_Dumb.thy
@@ -10,14 +10,21 @@ instantiation dumb_base :: absstate
 begin
   definition "\<top> \<equiv> Any"
   definition "\<bottom> \<equiv> Any"
+  definition "is_bot_dumb_base (a::dumb_base) \<equiv> True"
   fun less_eq_dumb_base :: "dumb_base \<Rightarrow> dumb_base \<Rightarrow> bool" where "less_eq_dumb_base _ _ \<longleftrightarrow> True"
   fun less_dumb_base :: "dumb_base \<Rightarrow> dumb_base \<Rightarrow> bool" where "less_dumb_base _ _ \<longleftrightarrow> False"
   fun sup_dumb_base :: "dumb_base \<Rightarrow> dumb_base \<Rightarrow> dumb_base" where "sup_dumb_base _ _  = Any"
   fun inf_dumb_base :: "dumb_base \<Rightarrow> dumb_base \<Rightarrow> dumb_base" where "inf_dumb_base _ _  = Any"
   fun Sup_dumb_base :: "dumb_base set \<Rightarrow> dumb_base" where "Sup_dumb_base _ = Any"
   fun Inf_dumb_base :: "dumb_base set \<Rightarrow> dumb_base" where "Inf_dumb_base _ = Any"
-instance by standard (auto simp: dumb_base_is_dumb)
+instance by standard (auto simp: dumb_base_is_dumb is_bot_dumb_base_def)
 end
+
+(*instantiation dumb_base :: equal
+begin
+definition "HOL.equal (a::dumb_base) b \<longleftrightarrow> True"
+instance sorry
+end*)
 
 type_synonym dumb = "dumb_base option"
 
@@ -43,7 +50,7 @@ fun dumb_step_direct :: "dumb astep" where
   "dumb_step_direct HALT ipc ins pc = None" |
   "dumb_step_direct _ ipc ins pc = (if pc = Suc ipc then Some Any else None)"
 
-lemma dumb_step_direct_eq: "dumb_step = dumb_step_direct"
+lemma dumb_step_direct_eq[code]: "dumb_step = dumb_step_direct"
 proof -
   have "dumb_step op ipc ins pc = dumb_step_direct op ipc ins pc" for op ipc ins pc
   proof(cases ins)
